wip, remain: `counterframe` is weak-transitive

Foundation/Modal/Kripke/AxiomFourN.lean
@@ -1,52 +1,44 @@
 import Foundation.Modal.Kripke.AxiomGeach
 import Foundation.Modal.Kripke.Filtration
-import Foundation.Vorspiel.Relation.Iterate
-
-
-section
-
-variable {n : ℕ+}  {α : Type u} {rel : α → α → Prop}
-
-def WeakTransitive (n : ℕ+) (rel : α → α → Prop) := ∀ x y, (Rel.iterate rel (n + 1)) x y → (Rel.iterate rel n) x y
-
-@[simp]
-lemma weak_transitive_one_transitive : (WeakTransitive 1 rel) ↔ Transitive rel := by
-  simp only [WeakTransitive, PNat.val_ofNat, Nat.reduceAdd, Rel.iterate.iff_succ, Rel.iterate.iff_zero, exists_eq_right, forall_exists_index, and_imp, Transitive];
-  constructor;
-  . intro h x y z; apply h;
-  . intro h x y z; apply h;
-
-class IsWeakTrans (n) (α) (rel : α → α → Prop) : Prop where
-  weakTrans : WeakTransitive n rel
-
-instance [IsWeakTrans n _ rel] : IsGeachConfluent ⟨0, n + 1, n, 0⟩ _ rel := ⟨by
-  suffices ∀ ⦃x y z : α⦄, x = y → ∀ (x_1 : α), rel x x_1 → Rel.iterate rel n x_1 z → Rel.iterate rel n y z by
-    simpa [GeachConfluent];
-  rintro x _ y rfl u Rxw Rwz;
-  apply IsWeakTrans.weakTrans;
-  use u;
-⟩
-
-instance [IsGeachConfluent ⟨0, n + 1, n, 0⟩ _ rel] : IsWeakTrans n _ rel := ⟨by
-  rintro x y ⟨u, Rxu, Ruy⟩;
-  have : ∀ u, rel x u → Rel.iterate rel (↑n) u y → Rel.iterate rel (↑n) x y := by
-    simpa using @IsGeachConfluent.geachean (g := ⟨0, n + 1, n, 0⟩) (R := rel) _ _ x x y;
-  apply this u Rxu Ruy;
-⟩
-
-end
 
 
 namespace LO.Modal
 
 open Kripke
-open IsGeachConfluent
 
 namespace Kripke
 
-variable {n : ℕ+}
+namespace Frame
 
-lemma validate_axiomFourN_of_weak_transitive {F : Kripke.Frame} [IsWeakTrans n _ F.Rel] : F ⊧ (Axioms.FourN n (.atom 0)) := validate_AxiomGeach_of_GeachConfluent (g := ⟨0, n + 1, n, 0⟩)
+variable {F : Frame} {n : ℕ+}
+
+class IsWeakTransitive (F : Kripke.Frame) (n : ℕ+) where
+  weak_trans : ∀ ⦃x y : F⦄, x ≺^[n + 1] y → x ≺^[n] y
+
+instance [F.IsPiecewiseStronglyConnected] : F.IsPiecewiseConnected := inferInstance
+
+lemma weak_trans [F.IsWeakTransitive n] : ∀ {x y : F.World}, x ≺^[n + 1] y → x ≺^[n] y := by
+  apply IsWeakTransitive.weak_trans
+
+instance [F.IsGeachConvergent ⟨0, n + 1, n, 0⟩] : F.IsWeakTransitive n := ⟨by
+  rintro x y ⟨u, Rxu, Ruy⟩;
+  have : ∀ u, x ≺ u → u ≺^[n] y → x ≺^[n] y := by
+    simpa using @IsGeachConvergent.gconv (g := ⟨0, n + 1, n, 0⟩) (F := F) _ x x y;
+  apply this u Rxu Ruy;
+⟩
+instance [F.IsWeakTransitive n] : F.IsGeachConvergent ⟨0, n + 1, n, 0⟩ := ⟨by
+  suffices ∀ ⦃x y z : F⦄, x = y → ∀ (x_1 : F), x ≺ x_1 → x_1 ≺^[n] z → y ≺^[n] z by simpa using this;
+  rintro x _ y rfl u Rxw Rwz;
+  apply IsWeakTransitive.weak_trans;
+  use u;
+⟩
+
+end Frame
+
+
+variable {F : Kripke.Frame} {n : ℕ+}
+
+lemma validate_AxiomFourN_of_weakTransitive [F.IsWeakTransitive n] : F ⊧ (Axioms.FourN n (.atom 0)) := validate_axiomGeach_of_isGeachConvergent (g := ⟨0, n + 1, n, 0⟩)
 
 namespace Canonical
 
@@ -58,9 +50,7 @@ open Entailment
 open MaximalConsistentTableau
 open canonicalModel
 
-instance isWeakTrans [Entailment.HasAxiomFourN n 𝓢] : IsWeakTrans n _ (canonicalFrame 𝓢).Rel := by
-  have := isGeachConfluent (g := ⟨0, n + 1, n, 0⟩) (𝓢 := 𝓢);
-  infer_instance;
+instance [Entailment.HasAxiomFourN n 𝓢] : (canonicalFrame 𝓢).IsWeakTransitive n := by infer_instance;
 
 end Canonical
 
